\section{Proof of Theorem \ref{thm:1-1}}\label{sec:pfThm}
We are ready to complete the proof of Theorem \ref{thm:1-1}.
The substitution of $x = 1$ in Theorem \ref{main-thm} yields:
\begin{proposition}
  \label{cor:1}{\tmdummy}
  
%%  \begin{multline}
%%    \displaystyle\int_{- 1}^1 \displaystyle\int_{- 1}^1 | s + t |^{2 c-1} (1 - s^2)^{a-1
%%	    } (1 - t^2)^{b-1} C_{\ell}^{a-\frac{1}{2}} (s)
%%	    C_m^{b-\frac{1}{2}} (t) d s d t   \\
%%	    \displaystyle = \frac{(\frac{1}{2}- c)_{\frac{\ell + m}{2}} (- 1)^{\frac{\ell + m}{2}}
%%    \pi^{\frac{1}{2}} (2a-1)_{\ell} (2 b-1)_m \Gamma \left( 
%%    a \right) \Gamma \left( b \right) \Gamma \left(
%%    c \right) \Gamma (a+b+2c-1)}{\ell !m!
%%    \Gamma \left( a+c + \frac{\ell - m}{2}  \right) \Gamma \left(
%%    b+c - \frac{\ell - m}{2}  \right) \Gamma \left( a+b +
%%    c + \frac{\ell + m}{2} -\frac{1}{2} \right)} . 
%%    \end{multline}
    \begin{multline}
    \displaystyle\int_{- 1}^1 \displaystyle\int_{- 1}^1 | s + t |^{2 \nu} (1 - s^2)^{\lambda -
    \frac{1}{2}} (1 - t^2)^{\mu - \frac{1}{2}} C_{\ell}^{\lambda} (s)
    C_m^{\mu} (t) d s d t   =a^{\ell,m}_{\lambda,\mu,\nu}v_\ell^\lambda v^\mu_m\\
    \displaystyle = \frac{(- \nu)_{\frac{\ell + m}{2}} (- 1)^{\frac{\ell + m}{2}}
    \pi^{\frac{1}{2}} (2 \lambda)_{\ell} (2 \mu)_m \Gamma \left( \lambda +
    \frac{1}{2} \right) \Gamma \left( \mu + \frac{1}{2} \right) \Gamma \left(
    \nu + \frac{1}{2} \right) \Gamma (\lambda + \mu + 2 \nu + 1)}{\ell !m!
    \Gamma \left( \lambda + \nu + \frac{\ell - m}{2} + 1 \right) \Gamma \left(
    \mu + \nu - \frac{\ell - m}{2} + 1 \right) \Gamma \left( \lambda + \mu +
    \nu + \frac{\ell + m}{2} + 1 \right)}  \label{eqn:cor:1} .
  \end{multline}
\end{proposition}
%8 star
Owing to Proposition \ref{prop:1718105}, we can deduce
Theorem \ref{thm:1-1}
from Proposition \ref{cor:1}
under a slightly weaker assumption that $\lambda,\mu\in\R$ and $\nu\in\C$ satisfy\begin{equation*}
	\lambda,\mu>-\frac{1}{2};\quad\lambda,\mu\neq0;\quad2\Re \nu>\lambda+\mu+2,
\end{equation*}because for any $m,n\in\N$ with $m\le\lambda+2$ and $n\le\mu+2$, we have\begin{equation*}
	\frac{\partial^{m+n}}{\partial s^m\partial t^n}\myabs{s+t}^{2\nu}\in L^2\left( (-1,1)^2,(1-s^2)^{\lambda+m}(1-t^2)^{\mu+n}dsdt \right).
\end{equation*}
Hence Theorem \ref{thm:1-1} is proved.
