\documentclass[pdf,notes]{beamer}
\mode<presentation>{\usetheme[secheader]{Boadilla}}

\usepackage{mathtools}
\usepackage{xypic}
\usepackage[all,cmtip]{xy}
\usepackage{mystyle}
\includecomment{versiona}
\usepackage{xeCJK}
\usepackage{lpic}
\usefonttheme{professionalfonts}
\usepackage{etoolbox}

\newcommand{\red}[1]{{\color[rgb]{0.6,0,0}#1}}
\setbeamertemplate{theorems}[numbered] 

\usepackage{tikz}
\usetikzlibrary{shapes,arrows,patterns}
\renewcommand{\implies}{\Rightarrow}
\newcommand{\Sol}{\mathcal{S}\mbox{ol}}
\newcommand{\Ind}{\mbox{\normalfont Ind}}
\newcommand{\Hom}{\mbox{\normalfont Hom}}
\newcommand{\D}{\mathcal{D}}
\newcommand{\A}{\mathcal{A}}
\newcommand{\Co}{\mathbb{C}}
\newcommand{\X}{\mathbb{X}}
\renewcommand{\setminus}{\backslash}
\newcommand{\nin}{\not\in}
\newcommand{\tmop}[1]{\ensuremath{\operatorname{#1}}}
\newcommand{\tmtextbf}[1]{{\bfseries{#1}}}
\newcommand{\tmtextit}[1]{{\itshape{#1}}}
\newcommand{\mss}{//}
\newcommand{\mbb}{\backslash\backslash}
\newcommand{\mmm}{\mid\mid}
\catcode`\<=\active \def<{
\fontencoding{T1}\selectfont\symbol{60}\fontencoding{\encodingdefault}}
\catcode`\>=\active \def>{
\fontencoding{T1}\selectfont\symbol{62}\fontencoding{\encodingdefault}}
\newcommand{\assign}{:=}
\newcommand{\comma}{{,}}
\newcommand{\um}{-}
\newcommand{\sol}{\mathcal{S}ol(\R^{p,q};\lambda,\nu)}
\newcommand{\Op}{\mbox{\normalfont Op}}
\newcommand{\Res}{\operatorname{Res}\displaylimits}
\newcommand{\OpR}{\mbox{\it R}}

%%\makeatletter
%%\newenvironment<>{proofs}[1][\proofname]{\par\def\insertproofname{#1\@addpunct{.}}\usebeamertemplate{proof begin}#2}
%%{\usebeamertemplate{proof end}}
%%\makeatother

\newtheorem{prop}{命題}
\newtheorem*{prop*}{命題}
\newtheorem{remark}{注}
\newtheorem{cor}{系}

\AtBeginEnvironment{remark}{%
	    \setbeamercolor{block title}{bg=orange,fg=white}
		\setbeamercolor{block body}{bg=orange!20,fg=black}
}
\AtBeginEnvironment{fact}{%
	    \setbeamercolor{block title}{bg=green,fg=black}
		\setbeamercolor{block body}{bg=orange!20,fg=black}
}
\AtBeginEnvironment{cor}{%
	    \setbeamercolor{block title}{bg=blue,fg=white}
		\setbeamercolor{block body}{bg=orange!20,fg=black}
}

\setCJKmainfont[AutoFakeBold=true]{Hiragino Mincho Pro} %my Mac

\title[2つのゲーゲンバウアー多項式に\dots]{2つのゲーゲンバウアー多項式に関連する積分公式について\footnote{60 min talk}}

% A subtitle is optional and this may be deleted

\author[レオンチエフ・アレックス]{小林俊行\inst{1} \and \underline{レオンチエフ・アレックス}\inst{2}}

\institute[東大] % (optional, but mostly needed)
{
  \inst{1}%
  大学院数理科学研究科、カブリ数物連携宇宙研究機構\\
  東京大学
  \and
  \inst{2}%
  大学院数理科学研究科\\
  東京大学
  }

  \date[表現論とその周辺分野\dots]{RIMS共同研究（公開型）\\「表現論とその周辺分野の広がり」\\京都大学数理解析研究所}
% - Either use conference name or its abbreviation.
% - Not really informative to the audience, more for people (including
%   yourself) who are reading the slides online

\subject{表現論}

\begin{document}
\begin{frame}\titlepage\end{frame}

\begin{frame}{Outline}
	\tableofcontents
\end{frame}
\section{The Main Result}
\begin{frame}
	\begin{prop}\label{prop:exp-st-gg}
		\begin{equation}
			| s + t |^{2 \nu} = \sum_{\mbox{\scriptsize $\begin{array}[]{c}
			\ell, m = 0 \\ \ell + m : \tmop{even}
		\end{array}$}}^{\infty} a_{\lambda,\mu,\nu}^{\ell,m} C_\ell^{\lambda} (s) C_m^{\mu} (t),
			\label{eqn:exp-st-gg}
		\end{equation}
		{\scriptsize
		\begin{equation*}
	a_{\lambda,\mu,\nu}^{\ell,m}= \frac{ 2^{-2\nu}(\lambda + \ell) (\mu + m)  \Gamma (\lambda + \mu + 2 \nu + 1) \Gamma (\lambda)
  \Gamma (\mu)\Gamma \left( 2\nu +
1 \right)}{\Gamma \left( \lambda + \nu + \frac{\ell -
  m}{2} + 1 \right)  \Gamma \left( \mu + \nu -
  \frac{\ell - m}{2} + 1 \right) \Gamma \left( \lambda + \mu + \nu + \frac{\ell +
  m}{2} + 1 \right)\Gamma\left(  \nu+1-\frac{\ell+m}{2}\right)}
		\end{equation*}
	}
	\end{prop}
	Here, $C_{\ell}^\lambda(t)$ ($\lambda\in\mathbb{C},\ell\in\N$) is the Gegenbauer polynomial.
	\begin{remark}
		We could not find this formula in the literature.
	\end{remark}
\end{frame}
\begin{frame}
	\begin{figure}[h]
		\centering
\begin{lpic}[]{wanted(0.75)}
	\lbl[bl]{3,15; \large$\begin{array}[]{c}
		\mbox{\it Expansion of $| s + t |^{2 \nu}$}\\\\\mbox{ in the form} \\\\
	| s + t |^{2 \nu} =	\\\\
	\sum_{\mbox{\scriptsize $\begin{array}[]{c}
\ell, m = 0 \\	 l + m\in2\N
\end{array}$}}^{\infty}
		a_{\lambda, \mu, \nu}^{\ell, m} C_{\ell}^{\lambda} (s) C_m^{\mu} (t)
	\end{array}$} %dot 
		
	\end{lpic}
		\label{fig:wanted}
	\vspace{-0.5cm}
	\caption*{Can we find the {closed expression} for $a_{\lambda,\mu,\nu}^{\ell,m}$ \underline{in literature}???}
	\end{figure}
\end{frame}
\begin{frame}
	In fact, we can do more:
	\begin{prop}\label{prop:exp-stz-gg}
		  \label{thm:4}For $\tmop{Re} \lambda, \tmop{Re} \mu > - \frac{1}{2}$,
		    $\tmop{Re} (\nu) > 0$ and $-1 \leqslant z \leqslant 1$ the following holds:
		      \begin{eqnarray}
			          & | s + t z |^{2 \nu} \tmop{sgn}^{\frac{1 \pm 1}{2}} (s + t z) = \sum_{l,
					      m = 0 \mid l + m \equiv \frac{1 \pm 1}{2} \tmop{mod} 2}^{\infty} a_{l, m}
					          (z) C_l^{\lambda} (s) C_m^{\mu} (t), &  \nonumber\\
						      & a_{l, m} (z) = \frac{\Gamma \left( \nu + \frac{1}{2} \right) \Gamma
						      (\lambda) \Gamma (\mu) (\lambda + l) z^m }{(1 + \nu)_{- \frac{l + m}{2}} \sqrt{\pi} \Gamma
										      (\mu + m) \Gamma \left( \lambda + \nu + \frac{l - m}{2} + 1 \right)}&\nonumber
										      \\&\times{}_2 F_1 \left( \begin{array}{c}
								        \frac{l + m}{2} - \nu, \frac{m - l}{2} - \nu - \lambda\\
									      \mu + m + 1
									          \end{array} ; z^2 \right). & 
										          \nonumber
											    \end{eqnarray}
										    \end{prop}
\end{frame}
%%\section{Original motivation}
%%\newcommand{\mysbo}{A:\pi\kern-0.1cm\mid_{G'}\xrightarrow{G'}\tau}
%%{
%%\begin{frame}{Original Goal}
%%	\begin{block}
%%		
%%	\centerline{
%%		\xymatrixcolsep{0.5pc}
%%		\xymatrixrowsep{1pc}
%%		\xymatrix{G\ar@/_1pc/[d]&&\supset&&G'\ar@/^1pc/[d]&\\
%%			\pi&\ar[rr]^{A}&&\tau&&{\begin{array}[]{l}
%%				\\
%%		\mbox{ :\underline{infinitely-dimensional} representations}\\
%%		\mbox{ of \underline{noncompact} groups $G,G'$.}
%%		\end{array}}%
%%	}}
%%	\end{block}
%%	\setbeamercolor{block title}{bg=red!30,fg=black}
%%	\hspace{1cm}
%%	\vspace{-0.5cm}
%%	\begin{block}{Goal:}
%%%%		\[\begin{array}{cccl}
%%%%				G:=O(p+1,q+1)&\curvearrowright &\pi\mbox{ :infinitely-dimensional rep.}\\
%%%%		\bigcup&&&\\
%%%%		G':=O(p,q+1)&\curvearrowright &\tau\mbox{ :infinitely-dimensional rep.}
%%%%		\end{array}\]
%%		Classify all $G'$-intertwining operators $\mysbo$.
%%	\end{block}
%%\end{frame}
%%\begin{frame}{Idea}
%%	\begin{itemize}%[<+(1)->]
%%		\item Although $\pi$ and $\tau$ are realized on different spaces, we can define ``generalized eigenvalues'';
%%		\item it turns out that any $\mysbo$ is ``diagonal'';
%%		\item $\implies$ it would help to compute eigenvalues explicitly;
%%	\end{itemize}
%%\end{frame}
%%}
%%\begin{frame}
%%\begin{center}
%%	\begin{tikzpicture}
%%	\input{diagram.tex}
%%	\end{tikzpicture}
%%\end{center}
%%\end{frame}
%%\begin{frame}{Idea}
%%	\begin{itemize}%[<+(1)->]
%%		\item \ldots
%%		\item $\implies$ it would help to compute eigenvalues explicitly;
%%		\item $\mysbo$ are given by integral kernels 
%%		\item $\implies$ eigenvalues are given by integrals.
%%	\end{itemize}
%%\end{frame}
\section{What does it have to do with?}
\begin{frame}
	Proposition \ref{prop:exp-st-gg} is equivalent to the integral equality
	\begin{prop}
		\label{prop:int-st-gg}
		\begin{equation*}
			\int_{- 1}^1 \int_{- 1}^1 | s - t |^{2 \nu} (1 - s^2)^{\lambda - \frac{1}{2}}
			(1 - t^2)^{\mu - \frac{1}{2}} C_l^{\lambda} (s) C_m^{\mu} (t) d s d t
		\end{equation*}
		{\scriptsize
		\begin{equation}
			=\frac{(- \nu)_{\frac{l + m}{2}} (- 1)^{\frac{l - m}{2}} \pi^{\frac{1}{2}} (2
			\lambda)_l (2 \mu)_m \Gamma \left( \lambda + \frac{1}{2} \right) \Gamma \left(
			\mu + \frac{1}{2} \right) \Gamma \left( \nu + \frac{1}{2} \right) \Gamma
		(\lambda + \mu + 2 \nu + 1)}{l!m! \Gamma \left( \lambda + \nu + \frac{l -
		m}{2} + 1 \right) \Gamma \left( \mu + \nu - \frac{l - m}{2} + 1 \right) \Gamma
		\left( \lambda + \mu + \nu + \frac{l + m}{2} + 1 \right)}
			\label{eqn:int-st-gg}
			\tag{1$'$}
		\end{equation}
		}
	\end{prop}
\end{frame}
%%\section{What does it have to do with?}
\begin{frame}
	Furthermore,
	\begin{cor}\label{cor:int-xzy-hh}
		Taking $\ell=m=0$ in (the integral form of) Proposition \ref{prop:exp-stz-gg} and taking $\lambda,\mu\to\infty$ we arrive at:
		\begin{equation*}
			\begin{array}[]{c}
			\int_{- \infty}^{\infty} \int_{- \infty}^{\infty} | x - z y |^{2 \nu} e^{-
			x^2 - y^2} H_l (x) H_m (y) d x d y \\= (- \nu)_{\frac{l + m}{2}} (- 1)^{\frac{l
			- m}{2}} 2^{l + m} \pi^{\frac{1}{2}} \Gamma \left( \frac{1}{2} + \nu \right)
			(z^2 + 1)^{\nu - \frac{l + m}{2}} z^m .
			\end{array}
		\end{equation*}
	\end{cor}
	\begin{remark}
		The particular case $k=2$ of \underline{Mehta integral} follows from this.
	\end{remark}
	Even more,
\end{frame}
\begin{frame}[fragile]{Hierarchy}
\begin{tikzpicture}
\input{intdep.tex}
\end{tikzpicture}
\end{frame}
\begin{frame}
	Furthermore, making variable change $w=s-t$ in Corollary \ref{cor:int-xzy-hh} and taking $z=1$ we arrive at\footnote[frame]{FIXME: check correctness}:
	\begin{cor}
		The following holds:
		\begin{equation}
			\mathcal{M}(hr_n\ast hr_m)(s)=
			\left(  \frac{1-s}{2}\right)_{\frac{l + m}{2}} (- 1)^{\frac{l
			+ m}{2}}  \pi^{\frac{1}{2}} \Gamma \left( \frac{s}{2} \right)
			2^{\frac{s-3}{2} + \frac{l + m}{2}}.
%%			\begin{array}[]{c}
%%			\int_{- \infty}^{\infty} \int_{- \infty}^{\infty} | x - y |^{2 \nu} e^{-
%%			x^2 - y^2} H_l (x) H_m (y) d x d y \\= (- \nu)_{\frac{l + m}{2}} (- 1)^{\frac{l
%%			- m}{2}} 2^{l + m} \pi^{\frac{1}{2}} \Gamma \left( \frac{1}{2} + \nu \right)
%%			2^{\nu - \frac{l + m}{2}} .
%%			\end{array}
			\label{eqn:mellin-hh}
		\end{equation}
	\end{cor}
	where $\mathcal{M}(\cdot)$ is the Mellin transform\begin{equation*}
		\left\{ \mathcal{M}(f) \right\}(s)=\int_0^\infty x^{s-1}f(x)\;dx,
	\end{equation*}
	and $hr_n$ are \underline{Hermite-Rodriguez} functions \cite{mackenzie2003hermite}
	\begin{equation*}
		hr_n(x):=H_n(x)e^{-x^2}.
	\end{equation*}
	Applying inverse Mellin transform, we arrive at the well-known formula for convolution of Hermite-Rodriguez functions.
\end{frame}
\section{Proof}
\begin{frame}{Method 1 (simple, direct)}
	\begin{enumerate}
		\item It suffices to show Proposition \ref{prop:int-st-gg};
		\item In fact, \eqref{eqn:int-st-gg} follows from the special case $l=m=0$:
			{
				\footnotesize
			\begin{equation*}
				\kern-1cm\int_{- 1}^1 \int_{- 1}^1 | s - t |^{2 \nu} (1 - s^2)^{\lambda - \frac{1}{2}}
				(1 - t^2)^{\mu - \frac{1}{2}} d s d t = \frac{\pi^{\frac{1}{2}} \Gamma \left(
				\lambda + \frac{1}{2} \right) \Gamma \left( \mu + \frac{1}{2} \right) \Gamma
				\left( \nu + \frac{1}{2} \right) \Gamma (\lambda + \mu + 2 \nu + 1)}{\Gamma
				(\lambda + \nu + 1) \Gamma (\mu + \nu + 1) \Gamma (\lambda + \mu + \nu + 1)}
			\end{equation*}
		}
		via integration by parts;
		\item Upon change of variables $w=s-t$, the inner integral (in $w$) can be evaluated via \cite[ET II 186(9)]{gradshteinryzhik}:
		{
		\begin{equation*}
			\kern-1cm\int_0^u x^{\nu - 1} (x + \alpha)^{\lambda} (u - x)^{\mu - 1} d x =
			\alpha^{\lambda} u^{\mu + \nu - 1} B (\mu, \nu)_2 F_1 \left( - \lambda, \nu ;
			\mu + \nu ; - \frac{u}{\alpha} \right);
		\end{equation*}
	}
\item Taking the outer integral, we arrive at hypergeometric $_3F_2(;1)$ function which simplifies\footnote{TODO: elaborate} via Whipple's sum.
	\end{enumerate}
\end{frame}
\begin{frame}{Method 2 (simple, uses heavy machinery)}
	\begin{fact}[Carlson's Theorem]
		Suppose $f$ is an entire function defined on the right half-plane $\left\{ z\in\mathbb{C}\mid \Re(z)>0 \right\}$, such that:\begin{enumerate}
			\item $\exists C,\tau>0$, such that $\myabs{f(z)}\le C e^{\tau\myabs{z}}$ for all $z$ in right half-plane;
			\item $\exists C>0,c<\pi$, such that $\myabs{f(iy)}\le Ce^{c\myabs{y}}$ for all $y\in\R$;
			\item $f$ vanishes on positive integers $\N_+$.
		\end{enumerate}
		Then $f\equiv0$.
	\end{fact}
	Using this, \eqref{eqn:int-st-gg} can be deduced from the case $\nu\in\N_{+}$, which in turn follows after simple computations.
\end{frame}
\begin{frame}{Method 3 (harder, direct)}
	\begin{itemize}
		\item Prove Proposition \ref{prop:exp-stz-gg}
	\end{itemize}<++>
\end{frame}<++>
\begin{frame}[allowframebreaks]{References}
	\bibliographystyle{apalike}
	\nocite{Selberg:411367}
	\nocite{warnaar2010sl3}
	\nocite{dotsenko1985four}
	\nocite{tarasov2003selberg}
%%	\nocite{kobayashi2015symmetry}
%%	\nocite{kobayashi2015differential2}
%%	\nocite{kobayashi2016differential1}
%%	\nocite{kobayashi2014classification}
%%	\nocite{kobayashi2013finite}
%%	\nocite{kobayashi2015program}
\bibliography{intdep}
\end{frame}
\end{document}
